mutable_typed_shared_data: Use of seal_state/valid_sealed

theories/examples/mutable_typed_shared_data/invariants.v
@@ -5,32 +5,73 @@ Section invariants.
   Context {Σ:gFunctors} {memg:memG Σ} {regg:regG Σ} {sealsg: sealStoreG Σ}
           {nainv: logrel_na_invs Σ} `{MP: MachineParameters}.
 
-  Notation "a ↪ₐ w" := (mapsto (L := Addr) (V := Word) a DfracDiscarded w) (at level 20) : bi_scope.
-
-  Definition isIntSealed_int w': Word → iProp Σ :=
-    (λ w, (∃ a_cap, ⌜w = WCap RW a_cap (a_cap ^+ 1)%a a_cap⌝ ∗ a_cap ↪ₐ w' ∗ ⌜is_z w'⌝)%I).
-
-  Definition isIntSealed: Word → iProp Σ := (λ w, (∃ w', isIntSealed_int w' w))%I.
-
-  Definition seal_state ι addr τ {Hpers : ∀ w, Persistent (isIntSealed w)} : iProp Σ
-    := na_inv logrel_nais ι
-         (∃ τ_e, addr ↦ₐ WSealRange (true, true) τ τ_e τ ∗ ⌜(τ < τ_e)%ot⌝)%I
-       ∗ seal_pred τ isIntSealed.
-
   Definition sealN : namespace := nroot .@ "seal".
 
-  Lemma isIntSealed_alloc a_cap w:
-    a_cap ↦ₐ w ∗ ⌜is_z w⌝ ==∗ isIntSealed_int w (WCap RW a_cap (a_cap ^+ 1)%a a_cap).
+  Definition seal_state ι addr τ (φ: Addr → iPropI Σ) Φ {Hpers : ∀ w, Persistent (Φ w)} : iProp Σ :=
+    na_inv logrel_nais ι (φ addr) ∗ seal_pred τ Φ.
+
+  Definition valid_sealed w τ Φ :=
+    (∃ sb, ⌜w = WSealed τ sb⌝ ∗ ⌜∀ w : leibnizO Word, Persistent (Φ w)⌝ ∗ seal_pred τ Φ ∗ Φ (WSealable sb))%I.
+
+  Global Instance valid_sealed_persistent w o Φ: Persistent (valid_sealed w o Φ).
   Proof.
-    iIntros "(Ha & Hw)".
-    iMod (mapsto_persist with "Ha") as "#Ha".
-    iModIntro. iExists _; eauto.
+    Import uPred. (* exist_persistent *)
+
+    apply exist_persistent; intros sb.
+    unfold Persistent.
+    iIntros "(%Hw & %Hpers & #Hs & HP)".
+
+    (* use knowledge about persistence *)
+    iAssert (<pers> Φ (WSealable sb))%I with "[HP]" as "HP".
+    { by iApply Hpers. }
+
+    repeat (iApply persistently_sep_2; iSplitR); auto.
   Qed.
 
-  Instance isIntSealed_timeless w : Timeless (isIntSealed w).
-  Proof. apply _. Qed.
+  Lemma interp_valid_sealed sb o:
+    interp (WSealed o sb) -∗ ▷ ∃ Φ, valid_sealed (WSealed o sb) o Φ.
+  Proof.
+    iIntros "Hsl".
+    rewrite fixpoint_interp1_eq /=.
+    iDestruct "Hsl" as (Φ) "(%Hpers & Hpred & Hφ)".
+    iExists Φ, sb.
+    by repeat iSplit.
+  Qed.
 
-  Instance isIntSealed_persistent w : Persistent (isIntSealed w).
-  Proof. apply _. Qed.
+  Lemma seal_state_valid_sealed_pred_eq ι addr τ w φ Φ Φ' {Hpers : ∀ w, Persistent (Φ w)}:
+    seal_state ι addr τ φ Φ -∗ valid_sealed w τ Φ' -∗  (∀ w, ▷ (Φ w ≡ Φ' w)).
+  Proof.
+    iIntros "HsealLL Hvs".
+    iDestruct "HsealLL" as "[_ Hsp]".
+    iDestruct "Hvs" as (sb) "(_ & _ & Hsp' & _)".
+    iApply (seal_pred_agree with "Hsp Hsp'").
+  Qed.
 
 End invariants.
+
+Section invariants_int.
+  Context {Σ:gFunctors} {memg:memG Σ} {regg:regG Σ} {sealsg: sealStoreG Σ}
+          {nainv: logrel_na_invs Σ} `{MP: MachineParameters}.
+
+  Notation "a ↪ₐ w" := (mapsto (L := Addr) (V := Word) a DfracDiscarded w) (at level 20) : bi_scope.
+
+  Definition int_sealed: Word → iProp Σ :=
+    (λ w, (∃ a_cap w', ⌜w = WCap RW a_cap (a_cap ^+ 1)%a a_cap⌝ ∗ a_cap ↪ₐ w' ∗ ⌜is_z w'⌝)%I).
+
+  Definition seal_state_int ι addr τ: iProp Σ :=
+    seal_state ι addr τ (λ addr, ∃ v, addr ↦ₐ v ∗ ⌜is_z v⌝)%I int_sealed.
+  Definition valid_sealed_int w τ := valid_sealed w τ int_sealed.
+
+  Instance int_sealed_timeless w : Timeless (int_sealed w).
+  Proof. apply _. Qed.
+
+  Instance int_sealed_persistent w : Persistent (int_sealed w).
+  Proof. apply _. Qed.
+
+  Lemma seal_state_int_valid_sealed_pred_eq ι addr τ w Φ:
+    seal_state_int ι addr τ -∗ valid_sealed w τ Φ -∗  (∀ w, ▷ (int_sealed w ≡ Φ w)).
+  Proof.
+    iApply seal_state_valid_sealed_pred_eq.
+  Qed.
+
+End invariants_int.
